\documentclass{article}
\usepackage[utf8]{inputenc}
\usepackage{setspace}
\usepackage{tikz}
\usetikzlibrary{positioning}
\usepackage{amsfonts}
\usepackage{amssymb}
\usepackage{amsmath}
\usepackage{amsthm}
\usepackage{systeme}
\usepackage{mathtools}
\usepackage{hyperref}
\usepackage{venndiagram}
\usepackage{pgfplots}
\usetikzlibrary{pgfplots.statistics}
\pgfplotsset{compat=newest}

\begin{document}
\section*{Question 1}

~

\begin{proof}
    \begin{align*}
        &\text{Suppose: }b>a\\
        &\varepsilon \coloneqq \frac{b-a}{2}\\
        &b>a\implies \frac{b-a}{2}>0\\
        \Rightarrow&\varepsilon >0\\
        &b-\varepsilon =b-\frac{b-a}{2}=\frac{a+b}{2}\\
        &\frac{a+b}{2}>a\\
        \Rightarrow&b-\varepsilon >a\\
        &b-\varepsilon >a\nLeftrightarrow a>b-\varepsilon\\
        \Rightarrow&a\geqslant b\\
    \end{align*}
\end{proof}

\newpage

\section*{Question 2}

~

\begin{proof}
    \begin{align*}
        &a^2-b^2=a^2+ab-b^2-ab\\
        &=a(a+b)-b(a+b)\\
        &=(a+b)(a-b)\\
        &b\coloneqq -a\\
        \Rightarrow&a^2-(-a)^2=(a+(-a))(a-(-a))\\
        &=0\times (a+a)\\
        &=0\\
        \Rightarrow&a^2-(-a)^2=0\\
        \Rightarrow&(-a)^2=a^2\\
    \end{align*}
\end{proof}

\newpage

\section*{Question 3}

~

\begin{proof}
    \begin{align*}
        &\forall a,b\in \mathbb{R}:\\
        &\frac{1}{2}a,\frac{1}{2}b\in\mathbb{R} \\
        \Rightarrow&(\frac{1}{2}a-\frac{1}{2}b)^2\geqslant 0\\
        &\frac{1}{4}a^2-\frac{1}{2}ab+\frac{1}{4}b^2\geqslant0\\
        &\frac{1}{2}a^2+\frac{1}{2}b^2\geqslant \frac{1}{4}a^2+\frac{1}{2}ab+\frac{1}{4}b^2\\
        &\frac{1}{2}(a^2+b^2)\geqslant [\frac{1}{2}(a+b)]^2\\
        &\\
        &\frac{1}{2}(a^2+b^2)= [\frac{1}{2}(a+b)]^2\implies a=b:\\
        &\frac{1}{2}a^2+\frac{1}{2}b^2-[\frac{1}{2}(a+b)]^2=0\\
        &\frac{1}{2}a^2+\frac{1}{2}b^2-(\frac{1}{4}a^2+\frac{1}{2}ab+\frac{1}{4}b^2)\\
        &\frac{1}{4}a^2-\frac{1}{2}ab+\frac{1}{4}b^2=0\\
        &[\frac{1}{2}(a-b)]^2=0\\
        &a-b=0\\
        &a=b\\
        \Rightarrow&\frac{1}{2}(a^2+b^2)= [\frac{1}{2}(a+b)]^2\implies a=b\\
        &\\
        &a=b\implies \frac{1}{2}(a^2+b^2)= [\frac{1}{2}(a+b)]^2:\\
        &LHS=\frac{1}{2}(a^2+a^2)=a^2\\
        &RHS=[\frac{1}{2}(a+a)]^2=a^2\\
        &LHS=RHS\\
        \Rightarrow&\frac{1}{2}(a^2+b^2)= [\frac{1}{2}(a+b)]^2\\
        \Rightarrow&a=b\implies \frac{1}{2}(a^2+b^2)= [\frac{1}{2}(a+b)]^2\\
        \Rightarrow&\frac{1}{2}(a^2+b^2)= [\frac{1}{2}(a+b)]^2\Leftrightarrow a=b\\
    \end{align*}
\end{proof}
\end{document}